proof/refine/PageTableDuplicates.thy
@@ -2786,7 +2786,7 @@ lemma hc_valid_duplicates'[wp]:
 
 lemma handleWait_valid_duplicates'[wp]:
   "\<lbrace>(\<lambda>s. vs_valid_duplicates' (ksPSpace s))\<rbrace> 
-  handleWait \<lbrace>\<lambda>r s. vs_valid_duplicates' (ksPSpace s)\<rbrace>"
+  handleWait isBlocking \<lbrace>\<lambda>r s. vs_valid_duplicates' (ksPSpace s)\<rbrace>"
   apply (simp add: handleWait_def cong: if_cong)
   apply (rule hoare_pre)
    apply wp
